invariants ex: more general identifier class - init

examples/invariants/DY.Example.Invariants.Uniqueness.Identifier.fst
@@ -26,8 +26,9 @@ type identifier = nat
 
 class has_identifier (state_t:Type) = {
   base: parseable_serializeable bytes state_t;
-  to_id: state_t -> identifier
+  to_id: state_t -> identifier;
 }
+
 
 
 (*** Generating a new Identifier ***)
@@ -152,3 +153,234 @@ p:principal -> tr:trace ->
 let new_idn_does_not_appear_in_full_state #state_t #hid p tr =
   let fst = access_full_state tr p in
   curr_max_id_largest #state_t to_id fst
+  
+(*** More general  ***)
+
+open Ord
+
+class identifier_ (id_t:eqtype) {|ord_leq id_t|} = {
+  initial_id: id_t;
+  next_id: id_t -> id_t;
+  next_id_larger: x:id_t -> Lemma (x `lt` next_id x)
+}
+
+// the main property: new_identifier > current max identifier
+class has_identifier_ (state_t:Type) (id_t:eqtype) {|ord_leq id_t|} {|identifier_ id_t|} = {
+  base_: parseable_serializeable bytes state_t;
+  to_id_: state_t -> id_t;
+}
+
+// returns Some only for sessions where all states can be successfully parsed
+let rec find_max_id_in_session_gen (#state_t:Type) (#id_t:eqtype) {|ord_leq id_t |} {|identifier_ id_t|} {|hid: has_identifier_ state_t id_t|} 
+    (sess:rev_list state_raw) 
+    : option id_t = 
+    match sess with
+    | Nil -> None
+    | Snoc rest state -> 
+        match parse state_t #hid.base_ state with
+        | None -> find_max_id_in_session_gen #state_t #_ #_ #_ #hid rest
+        | Some st -> (
+            match find_max_id_in_session_gen #state_t #_ #_ #_ #hid rest with
+            | None -> Some (to_id_ st)
+            | Some cur_max ->
+         Some (max (hid.to_id_ st) cur_max)
+        )
+
+
+// let prop_state_on (#a:Type) (#state_t:Type) {|ps_state : parseable_serializeable bytes state_t|} 
+//   (from_state: state_t  -> a) (p: a -> bool ) (state:state_raw) : prop =
+//   match parse state_t state with
+//   | None -> True
+//   | Some state -> p (from_state state)
+
+let forall_ids_gen  (#state_t:Type) (#id_t:eqtype) {|ord_leq id_t|} {|identifier_ id_t|} {|hid:has_identifier_ state_t id_t|}  
+   (sess:(session_raw)) (p: id_t -> bool) : prop =
+  forall_rev_list sess (fun state -> prop_state_on #_ #state_t #hid.base_ hid.to_id_ p state )
+
+
+let rec find_max_id_in_session_gen_none
+(#state_t:Type) (#id_t:eqtype) {|ord_leq id_t |} {|identifier_ id_t|} {|hid: has_identifier_ state_t id_t|} 
+    (sess:rev_list state_raw) 
+    : Lemma 
+    (requires None? (find_max_id_in_session_gen #state_t #id_t sess))
+    (ensures
+       forall_rev_list sess (fun st -> None? (parse state_t #hid.base_ st))
+    )
+= match sess with
+  | Nil -> ()
+  | Snoc rest st -> find_max_id_in_session_gen_none #state_t #id_t rest
+
+
+#push-options "--fuel 4 --ifuel 4"
+val max_id_in_session_largest_gen:
+  (#state_t:Type) -> (#id_t:eqtype) -> {|ord_leq id_t |} -> {|identifier_ id_t|} -> {| hid: has_identifier_ state_t id_t|} ->
+  sess:session_raw ->
+  Lemma 
+  ( let m_idn = find_max_id_in_session_gen #_ #_ #_ #_ #hid sess in
+    match m_idn with
+    | Some m_idn ->
+    forall_ids_gen #state_t sess (fun idn -> idn `leq` m_idn)
+    | None -> True
+  )
+let rec max_id_in_session_largest_gen #state_t #id_t #_ #_ #hid sess = 
+  let m_idn = find_max_id_in_session_gen #state_t #id_t sess in
+  match m_idn with
+  | None -> ()
+  | Some m_idn -> (
+  match sess with
+  | Snoc Nil state -> ()
+  | Snoc rest state -> 
+  max_id_in_session_largest_gen #state_t #id_t rest;
+      match parse state_t #hid.base_ state with
+      | None -> ()
+      | Some st ->
+      match find_max_id_in_session_gen #state_t #id_t rest with
+      | None -> ( find_max_id_in_session_gen_none #state_t #id_t rest
+)
+      | Some m_idn_rest -> (
+       max_is_largest (hid.to_id_ st) m_idn_rest
+))
+
+
+let rec find_max_id_in_full_state_gen (#state_t:Type) (#id_t:eqtype) {|ord_leq id_t|} {|identifier_ id_t|} {|hid: has_identifier_ state_t id_t|}  
+  (st:full_state_raw): option id_t = 
+    match st with
+    | [] -> None
+    | (_,sess)::rest ->
+        match (find_max_id_in_session_gen #state_t #id_t sess) with
+        | None -> (find_max_id_in_full_state_gen #state_t rest)
+        | Some sess_max_id -> 
+        match (find_max_id_in_full_state_gen #state_t rest) with
+        | None -> Some sess_max_id
+        | Some rest_max_id ->
+        Some (max sess_max_id rest_max_id)
+
+val compute_new_id_gen: (#state_t:Type) -> (#id_t:eqtype) -> {|ord_leq id_t|} -> {|identifier_ id_t|} -> {|hid: has_identifier_ state_t id_t|} -> principal -> traceful id_t
+let compute_new_id_gen #state_t #id_t #_ #hid prin =
+  let* opt_fst = get_full_state prin in
+  match opt_fst with
+  | None -> return (hid.initial_id)
+  | Some fst ->
+      match (find_max_id_in_full_state_gen #state_t #id_t fst) with
+      | None -> return hid.initial_id
+      | Some cur_max ->
+        return (
+        hid.next_id cur_max)
+
+
+
+let rec find_max_id_in_full_state_gen_none
+(#state_t:Type) (#id_t:eqtype) {|ord_leq id_t|} {|identifier_ id_t|} {|hid: has_identifier_ state_t id_t|}  
+  (f_st:full_state_raw):
+  Lemma
+  (requires None? (find_max_id_in_full_state_gen #state_t #id_t f_st))
+  (ensures
+     forall_sessions f_st 
+       (fun sid sess ->
+         forall_rev_list sess (fun st -> None? (parse state_t #hid.base_ st))
+       )
+  )
+  = match f_st with
+  | [] -> ()
+  | (sid,sess)::rest ->
+                    find_max_id_in_session_gen_none #state_t #id_t sess;
+                    find_max_id_in_full_state_gen_none #state_t #id_t rest
+
+#push-options "--z3rlimit 20"
+val curr_max_id_largest_gen :
+(#state_t:Type) -> (#id_t:eqtype) -> {|ord_leq id_t |} -> {|identifier_ id_t|} -> {|hid:has_identifier_ state_t id_t|}  ->
+  (to_id: (state_t -> id_t)) ->
+  fst: full_state_raw -> 
+  Lemma 
+  ( //let c_max = find_max_id_in_full_state_gen #state_t fst in
+   match find_max_id_in_full_state_gen #state_t fst with
+   | None -> True
+   | Some c_max ->
+    forall_sessions fst (fun sid sess -> forall_ids_gen #state_t #id_t sess  (fun idn -> idn `leq` c_max))
+  )
+let rec curr_max_id_largest_gen #state_t #id_t #_ #hid to_id fst =
+  match find_max_id_in_full_state_gen #state_t #id_t fst with 
+  | None -> ()
+  | Some c_max ->
+  match fst with
+  | [] -> ()
+  | (sid, sess) :: rest ->
+        max_id_in_session_largest_gen #state_t #id_t sess;
+        curr_max_id_largest_gen #state_t #id_t to_id rest;
+        match (find_max_id_in_session_gen #state_t #id_t sess) with
+        | None -> find_max_id_in_session_gen_none #state_t #id_t sess
+        | Some sess_max_id -> (
+            match (find_max_id_in_full_state_gen #state_t rest) with
+            | None -> 
+                find_max_id_in_full_state_gen_none #state_t #id_t rest
+            | Some rest_max_id -> (
+                max_is_largest sess_max_id rest_max_id
+        )
+  )
+#pop-options
+
+let id_does_not_appear_in_session_gen (#state_t:Type) (#id_t:eqtype) {|ord_leq id_t|} {|identifier_ id_t|} {|has_identifier_ state_t id_t|}  
+  (id:id_t) (sess:session_raw)  : prop =
+  forall_ids_gen #state_t #id_t sess (fun id' -> id <> id')
+
+
+let idn_does_not_appear_in_full_state_gen (#state_t:Type) (#id_t:eqtype) {|ord_leq id_t|} {|identifier_ id_t|} {|has_identifier_ state_t id_t|}  
+  (id:id_t) (fst:full_state_raw) : prop =
+  forall_sessions fst 
+    (fun _ sess -> id `id_does_not_appear_in_session_gen #state_t #id_t` sess)
+
+#push-options "--z3rlimit 30"
+/// The Main Property
+val new_idn_does_not_appear_in_full_state_gen:
+(#state_t:Type) -> (#id_t:eqtype) -> {|ord_leq id_t|} -> {|identifier_ id_t|} -> {|hid:has_identifier_ state_t id_t|}  ->
+p:principal -> tr:trace ->
+  Lemma
+  (requires has_full_state_for tr p
+  )
+  (ensures (
+    let (n_id,_) = compute_new_id_gen #state_t #id_t p tr in
+    let fst = access_full_state tr p in
+    n_id `idn_does_not_appear_in_full_state_gen #state_t` fst
+  ))
+let new_idn_does_not_appear_in_full_state_gen #state_t #id_t #_ #_ #hid p tr =
+  let f_st = access_full_state tr p in
+  let (n_id,_) = compute_new_id_gen #state_t #id_t p tr in
+  curr_max_id_largest_gen #state_t #id_t hid.to_id_ f_st;
+  match find_max_id_in_full_state_gen #state_t #id_t f_st with
+  | None ->
+      find_max_id_in_full_state_gen_none #state_t #id_t f_st
+  | Some curr_max -> (
+      next_id_larger curr_max
+      )
+#pop-options
+
+
+instance identifier_nat: identifier_ nat #ord_leq_nat = {
+  initial_id = 1;
+  next_id = (fun (i:nat) -> i + 1);
+  next_id_larger = (fun i -> ())
+}
+
+let rand_bytes = b:bytes{Rand? b}
+
+instance ord_leq_rand_bytes_time: ord_leq rand_bytes = {
+  leq_ = (fun (r1 r2:rand_bytes) ->
+    let Rand _ _ _ t1 = r1 in
+    let Rand _ _ _ t2 = r2 in
+    t1 <= t2
+  );
+  refl = (fun _ -> ());
+  total_ = (fun _ _ -> ());
+  // anti_symm = (fun _ _ -> ());
+  trans = (fun _ _ _ -> ())
+  
+}
+
+instance identifier_rand (u:usage) (l:label) (len:nat{len <> 0}): identifier_ rand_bytes #ord_leq_rand_bytes_time = {
+  initial_id = (Rand u l len 0);
+  next_id = (fun (r:rand_bytes) -> 
+    let Rand u l len t = r in
+    Rand u l len (t+1)
+  );
+  next_id_larger = (fun r -> ())
+}
