examples/invariants/DY.Example.Invariants.Uniqueness.fst
@@ -61,9 +61,18 @@ instance has_identifier_p_state_2: has_identifier p_state = {
   to_id = fun state -> state.idn2
 }
 
+
+open Ord
+
+instance has_identifier__p_state_1: has_identifier_ p_state nat #ord_leq_nat #identifier_nat  = {
+   base_ = parseable_serializeable_bytes_p_state;
+   to_id_ = (fun state -> state.idn1);
+}
+
+
 val new_idn1: principal -> traceful nat
 let new_idn1 prin = 
-  compute_new_id #p_state #has_identifier_p_state_1 prin
+  compute_new_id_gen #p_state #nat #_ #_ #has_identifier__p_state_1 prin
 
 val new_idn2: principal -> traceful nat
 let new_idn2 prin = 
@@ -334,4 +343,17 @@ let rec session_parse_all
        else session_parse_all init p sid st
      )
      ))
-   
+
+#push-options "--fuel 3"
+let _ =
+  let state1 = S 1 3 0 in
+  let state2 = S 5 7 3 in
+  let sess1 = (Snoc Nil (serialize p_state state1)) in
+  let sess2 = Snoc sess1 (serialize p_state state2) in
+  assert(find_max_id_in_session_gen #_ #_ #_ #_ #has_identifier__p_state_1 Nil = None);
+  assert(find_max_id_in_session_gen #_ #_ #_ #_ #has_identifier__p_state_1 sess1 = Some (1 <: nat));
+  assert(find_max_id_in_session_gen #_ #_ #_ #_ #has_identifier__p_state_1 sess2 = Some (5 <: nat));
+  let sid1 = {the_id = 1} in
+  let sid2 = {the_id = 2} in
+  let full_st = [(sid1, sess1); (sid2, sess2)] in
+  assert(find_max_id_in_full_state_gen #_ #_ #_ #_ #has_identifier__p_state_1 full_st = Some (5 <: nat))
