examples/invariants/Ord.fst
@@ -1,0 +1,130 @@
+module Ord
+
+/// The Ord Typeclass
+/// -----------------
+///
+/// * total order defined by a "less or equal" operator ``leq_``
+/// * containing proofs that ``leq_`` is a total order
+///   (reflexivity ``refl``, totality ``total_``, anti-symmetry ``anti_symm``, transitivity ``trans`` )
+
+class ord_leq (a:eqtype) =
+  { leq_: a -> a -> bool
+  ; refl: (x:a) -> Lemma (x `leq_` x)
+  ; total_: (x:a) -> (y:a) -> Lemma (x `leq_` y \/ y `leq_` x)
+  //; anti_symm: (x:a) -> (y:a) -> Lemma (x `leq_` y /\ y `leq_` x ==> x = y)
+  ; trans: (x:a) -> (y:a) -> (z:a) ->  Lemma (x `leq_` y /\ y `leq_` z ==> x `leq_` z)
+  }
+
+
+/// comparison functions derived from ``leq_``
+/// ~~~~~~~~~~~~~~~~~~~~~~~~~~~~~~~~~~~~~~~~~~~
+///
+/// corresponding to "<", "<=", ">" and ">="
+
+let lt (#a:eqtype){|ord_leq a|} (x y : a) : bool =
+  match (leq_ x y, x = y) with
+  | (true, false) -> true
+  | _ -> false
+
+let leq (#a:eqtype){|ord_leq a|} (x y : a) : bool = leq_ x y
+
+let lt_implies_leq {|ord_leq 'a|} (x y : 'a) :
+  Lemma 
+  (requires x `lt` y)
+  (ensures x `leq` y /\ x <> y)
+  [SMTPat (x `lt` y)]
+  = ()
+
+let leq_is_lt_or_equal {|ord_leq 'a|} (x y : 'a) :
+  Lemma
+  (requires
+     x `leq` y
+  )
+  (ensures
+     x `lt` y
+     \/ x = y
+  )
+  [SMTPat (x `leq` y)]
+  = ()
+
+/// the total order properties as separate lemmas
+/// (needed for helpful SMTPats)
+
+let reflexivity {|ord_leq 'a |} (x : 'a)
+  : Lemma (x `leq` x)
+    [SMTPat (x `leq` x)]
+  = refl x
+
+let totality {| ord_leq 'a |} (x y : 'a)
+  : Lemma (x `leq` y \/ y `leq` x)
+  [SMTPat (x `leq` y); SMTPat (y `leq` x)]
+  = total_ x y
+
+// let anti_symmetry #a {| oa: ord_leq a |} (x y : a)
+//   : Lemma (x `leq` y /\ y `leq` x ==> x = y)
+//   [SMTPat (leq #a #oa x  y)] //; SMTPat (y `leq` x)]
+//  = anti_symm x y
+
+let transitivity {| ord_leq 'a |} (x y z : 'a)
+  : Lemma (x `leq` y /\ y `leq` z ==> x `leq` z)
+  [SMTPat (x `leq` y); SMTPat (y `leq` z)]
+  = trans x y z
+
+let transitivity_forall #a {| ord_leq a |} unit
+  : Lemma (forall (x y z : a). x `leq` y /\ y `leq` z ==> x `leq` z )
+= ()
+
+let transitivity_lt {| ord_leq 'a |} (x y z : 'a)
+  : Lemma (x `lt` y /\ y `lt` z ==> x `lt` z)
+  [SMTPat (x `lt` y); SMTPat (y `lt` z)]
+  = admit()
+
+let transitivity_leq_lt {|ord_leq 'a|} (x y z : 'a)
+  : Lemma 
+    (requires
+       x `leq` y /\ y `lt` z
+    )
+    (ensures
+       x `lt` z
+    )
+    = () 
+
+
+let lt_not_eq {|ord_leq 'a|} (x y : 'a)
+  : Lemma 
+    (requires x `lt` y)
+    (ensures x <> y)
+    [SMTPat (x `lt` y)]
+    = ()
+
+let max {| ord_leq 'a |} (x y : 'a) =
+  if x `leq` y then y else x
+
+let max_is_largest {|ord_leq 'a|} (x y :'a) :
+  Lemma (x `leq` max x y /\ y `leq` max x y)
+  = ()
+
+/// Instances
+/// ---------
+
+/// Int
+/// ~~~
+
+instance ord_leq_int : ord_leq int =
+  { leq_ = (<=)
+  ; refl = (fun _ -> ())
+  ; total_ = (fun _ _ -> ())
+  // ; anti_symm = (fun _ _ -> ())
+  ; trans = (fun _ _ _ -> ())
+  }
+
+/// Nat
+/// ~~~
+
+instance ord_leq_nat : ord_leq nat =
+  { leq_ = (<=)
+  ; refl = (fun _ -> ())
+  ; total_ = (fun _ _ -> ())
+  // ; anti_symm = (fun _ _ -> ())
+  ; trans = (fun _ _ _ -> ())
+  }
